PlutusCore formalization: new ByteString representation based on String type

PlutusCore/String/Basic.lean
@@ -19,16 +19,97 @@ def appendString (s1 : String) (s2 : String) : String := s1 ++ s2
 
 def equalsString (s1 : String) (s2 : String) : Bool := s1 == s2
 
+def utf8EncodeChar (c : Char) : List Char :=
+  let v := c.val
+  if v ≤ 0x7f then
+    [c]
+  else if v ≤ 0x7ff then
+    [Char.ofUInt8 ((v >>>  6).toUInt8 &&& 0x1f ||| 0xc0),
+     Char.ofUInt8 (v.toUInt8 &&& 0x3f ||| 0x80)]
+  else if v ≤ 0xffff then
+    [Char.ofUInt8 ((v >>> 12).toUInt8 &&& 0x0f ||| 0xe0),
+     Char.ofUInt8 ((v >>>  6).toUInt8 &&& 0x3f ||| 0x80),
+     Char.ofUInt8 (v.toUInt8 &&& 0x3f ||| 0x80)]
+  else
+    [Char.ofUInt8 ((v >>> 18).toUInt8 &&& 0x07 ||| 0xf0),
+     Char.ofUInt8 ((v >>> 12).toUInt8 &&& 0x3f ||| 0x80),
+     Char.ofUInt8 ((v >>>  6).toUInt8 &&& 0x3f ||| 0x80),
+     Char.ofUInt8 (v.toUInt8 &&& 0x3f ||| 0x80)]
+
 /-- Coverts String to ByteString using utf8 encoding -/
-def encodeUtf8 (s : String) : ByteString := s.toUTF8
+def encodeUtf8 (s : String) : ByteString := ⟨⟨s.data.flatMap utf8EncodeChar⟩⟩
+
+def utf8DecodeChar? (a : List Char) (i : Nat) : Option Char := do
+  let u ← a[i]?
+  let c := u.toUInt8
+  if c &&& 0x80 == 0 then
+    some ⟨c.toUInt32, .inl (Nat.lt_trans c.toBitVec.isLt (by decide))⟩
+  else if c &&& 0xe0 == 0xc0 then
+    let u1 ← a[i+1]?
+    let c1 := u1.toUInt8
+    guard (c1 &&& 0xc0 == 0x80)
+    let r := ((c &&& 0x1f).toUInt32 <<< 6) ||| (c1 &&& 0x3f).toUInt32
+    guard (0x80 ≤ r)
+    -- TODO: Prove h from the definition of r once we have the necessary lemmas
+    if h : r < 0xd800 then some ⟨r, .inl ((UInt32.lt_ofNat_iff (by decide)).1 h)⟩ else none
+  else if c &&& 0xf0 == 0xe0 then
+    let u1 ← a[i+1]?
+    let u2 ← a[i+2]?
+    let c1 := u1.toUInt8
+    let c2 := u2.toUInt8
+    guard (c1 &&& 0xc0 == 0x80 && c2 &&& 0xc0 == 0x80)
+    let r :=
+      ((c &&& 0x0f).toUInt32 <<< 12) |||
+      ((c1 &&& 0x3f).toUInt32 <<< 6) |||
+      (c2 &&& 0x3f).toUInt32
+    guard (0x800 ≤ r)
+    -- TODO: Prove `r < 0x110000` from the definition of r once we have the necessary lemmas
+    if h : r < 0xd800 ∨ 0xdfff < r ∧ r < 0x110000 then
+      have :=
+        match h with
+        | .inl h => Or.inl ((UInt32.lt_ofNat_iff (by decide)).1 h)
+        | .inr h => Or.inr ⟨(UInt32.ofNat_lt_iff (by decide)).1 h.left, (UInt32.lt_ofNat_iff (by decide)).1 h.right⟩
+      some ⟨r, this⟩
+    else
+      none
+  else if c &&& 0xf8 == 0xf0 then
+    let u1 ← a[i+1]?
+    let u2 ← a[i+2]?
+    let u3 ← a[i+3]?
+    let c1 := u1.toUInt8
+    let c2 := u2.toUInt8
+    let c3 := u3.toUInt8
+    guard (c1 &&& 0xc0 == 0x80 && c2 &&& 0xc0 == 0x80 && c3 &&& 0xc0 == 0x80)
+    let r :=
+      ((c &&& 0x07).toUInt32 <<< 18) |||
+      ((c1 &&& 0x3f).toUInt32 <<< 12) |||
+      ((c2 &&& 0x3f).toUInt32 <<< 6) |||
+      (c3 &&& 0x3f).toUInt32
+    if h : 0x10000 ≤ r ∧ r < 0x110000 then
+      some ⟨r, .inr ⟨Nat.lt_of_lt_of_le (by decide) ((UInt32.ofNat_le_iff (by decide)).1 h.left), (UInt32.lt_ofNat_iff (by decide)).1 h.right⟩⟩
+    else none
+  else
+    none
 
 /-- Decodes a ByteString to String using utf8 decoding.
     An error is triggered when the ByteString is not uft8 encoded.
 -/
 def decodeUtf8 (bs : ByteString) : Except String String :=
- if h : String.validateUTF8 bs
- then pure (String.fromUTF8 bs h)
- else throw "decodeUtf8: invalid ByteString"
+  loop 0 bs.length bs.data.toList ""
+where
+  loop (i : Nat) (e : Nat) (bs : List Char) (acc : String) : Except String String :=
+    if _h : i < e then
+      match utf8DecodeChar? bs i with
+      | none => throw "decodeUtf8: invalid ByteString"
+      | some c =>
+          loop (i + c.utf8Size) e bs (acc.push c)
+    else pure acc
+  termination_by e - i
+  decreasing_by
+    have := Nat.sub_lt_sub_left _h (Nat.add_lt_add_left c.utf8Size_pos i)
+    decreasing_tactic
+
+-- exact Nat.sub_lt_sub_left ‹_› (Nat.lt_add_of_pos_right c.utf8Size_pos)
 
 end PlutusCore.StringInternal
 
@@ -38,7 +119,10 @@ export PlutusCore.StringInternal
     decodeUtf8
     emptyString
     encodeUtf8
+    decodeUtf8
     equalsString
+    utf8EncodeChar
+    utf8DecodeChar?
   )
 
 end PlutusCore.String
