PlutusCore/ByteString/Lemmas.lean
@@ -5,14 +5,22 @@ open PlutusCore.Integer
 
 /-! ## Theorem on ByteString representation and builtin functions. -/
 
-@[simp] theorem appendByteString_rfl (x y : ByteString) : appendByteString x y = x ++ y := rfl
+@[simp] theorem appendByteString_rfl (x y : ByteString) : appendByteString x y = x.data ++ y.data := rfl
 
 -- TODO: complete the following proofs
 theorem stringToByteString_lt_imp_lt (s1 s2 : String) :
-  ByteString.stringToByteString s1 < ByteString.stringToByteString s2 → s1 < s2 := by sorry
+  ByteString.stringToByteString s1 < ByteString.stringToByteString s2 → s1 < s2 := by
+    intro h;
+    unfold LT.lt at h;
+    simp [PlutusCore.ByteStringInternal.LTByteString, ByteString.stringToByteString] at h
+    assumption
 
 theorem lt_imp_stringToByteString_lt (s1 s2 : String) :
-  s1 < s2 → ByteString.stringToByteString s1 < ByteString.stringToByteString s2 := by sorry
+  s1 < s2 → ByteString.stringToByteString s1 < ByteString.stringToByteString s2 := by
+    intro h;
+    unfold LT.lt;
+    simp [PlutusCore.ByteStringInternal.LTByteString, ByteString.stringToByteString]
+    assumption
 
 @[simp] theorem stringToByteString_lt_iff_lt (s1 s2 : String) :
   ByteString.stringToByteString s1 < ByteString.stringToByteString s2 ↔ s1 < s2 := by
@@ -26,10 +34,9 @@ theorem lt_imp_stringToByteString_lt (s1 s2 : String) :
   then pure (ByteString.cons n.toNat.toUInt8 bs)
   else throw "consByteStringV2: invalid byte representation" := by rfl
 
-@[simp] theorem lengthOfByteString_rfl (bs : ByteString) : lengthOfByteString bs = Int.ofNat bs.size := rfl
+@[simp] theorem lengthOfByteString_rfl (bs : ByteString) : lengthOfByteString bs = Int.ofNat bs.length := rfl
 
-@[simp] theorem size_cons (u : UInt8) (bs : ByteString) : (ByteString.cons u bs).size = 1 + bs.size := by
-  simp only
-  [ ByteString.cons, ByteArray.size, Array.size, Array.toList_append, List.length_append, List.length_singleton ]
+@[simp] theorem size_cons (u : UInt8) (bs : ByteString) : (ByteString.cons u bs).length = 1 + bs.length := by simp [ByteString.cons]
+
 
 end PlutusCore.ByteString
