PlutusCore/String/Lemmas.lean
@@ -9,44 +9,27 @@ open PlutusCore.ByteString (ByteString)
 
 @[simp] theorem equalsString_rfl (x y : String) : equalsString x y = (x == y) := rfl
 
-@[simp] theorem encodeUft8_rfl (x : String) : encodeUtf8 x = x.toUTF8 := rfl
-
-@[simp] theorem decodeUtf8_rfl (bs : ByteString) :
-  decodeUtf8 bs =
-    if h : String.validateUTF8 bs
-    then pure (String.fromUTF8 bs h)
-    else throw "decodeUtf8: invalid ByteString"
-  := rfl
-
--- TODO : complete the following proofs
-theorem utf8EncodeChar_lt_imp_lt (c1 c2 : Char) :
-    String.utf8EncodeChar c1 < String.utf8EncodeChar c2 → c1 < c2 := by sorry
+-- -- TODO : complete the following proofs
+theorem utf8EncodeChar_lt_imp_lt (c1 c2 : Char) : utf8EncodeChar c1 < utf8EncodeChar c2 → c1 < c2 := by sorry
 
 theorem lt_imp_utf8EncodeChar_lt (c1 c2 : Char) :
-    c1 < c2 → String.utf8EncodeChar c1 < String.utf8EncodeChar c2 := by sorry
+    c1 < c2 → utf8EncodeChar c1 < utf8EncodeChar c2 := by sorry
 
 @[simp] theorem utff8EncodeChar_lt_iff_lt (c1 c2 : Char) :
-   String.utf8EncodeChar c1 < String.utf8EncodeChar c2 ↔ c1 < c2 := by
+   utf8EncodeChar c1 < utf8EncodeChar c2 ↔ c1 < c2 := by
    apply Iff.intro
    . apply utf8EncodeChar_lt_imp_lt
    . apply lt_imp_utf8EncodeChar_lt
 
-theorem toUTF8_lt_imp_lt (x y : String) : x.toUTF8 < y.toUTF8 → x < y := by sorry
-theorem lt_imp_toUTF8_lt (x y : String) : x < y → x.toUTF8 < y.toUTF8 := by sorry
+theorem toUTF8_lt_imp_lt (x y : String) : encodeUtf8 x < encodeUtf8 y → x < y := by sorry
 
-@[simp] theorem toUTF8_lt_iff_lt (x y : String) : x.toUTF8 < y.toUTF8 ↔ x < y := by
+theorem lt_imp_toUTF8_lt (x y : String) : x < y → encodeUtf8 x < encodeUtf8 y := by sorry
+
+@[simp] theorem toUTF8_lt_iff_lt (x y : String) : encodeUtf8 x < encodeUtf8 y ↔ x < y := by
   apply Iff.intro
   . apply toUTF8_lt_imp_lt
   . apply lt_imp_toUTF8_lt
 
-theorem encodeUft8_lt_imp_lt (x y : String) : encodeUtf8 x < encodeUtf8 y → x < y := by sorry
-
-theorem lt_imp_encodeUft8_lt (x y : String) : x < y → encodeUtf8 x < encodeUtf8 y := by sorry
-
-@[simp] theorem encodeUft8_lt_iff_lt (x y : String) : encodeUtf8 x < encodeUtf8 y ↔ x < y := by
-  apply Iff.intro
-  . apply encodeUft8_lt_imp_lt
-  . apply lt_imp_encodeUft8_lt
 
 
 end  PlutusCore.String
